Code/Preprocessing/Printing.v
@@ -1,0 +1,412 @@
+Require Import Prelude.Basics.
+Require Import Signature.
+Require Import String.
+Require Import List.
+Require Import Coq.Program.Equality.
+
+Local Open Scope string.
+
+(** * Pretty printing of terms *)
+
+(** ** Terms with named variables *)
+Inductive rawTm (V : Type) (F : Type) : Type :=
+| RawVar : V -> rawTm V F
+| RawBase : F -> rawTm V F
+| RawLam : V -> rawTm V F -> rawTm V F
+| RawApp : rawTm V F -> rawTm V F -> rawTm V F.
+
+Arguments RawVar {_ _} _.
+Arguments RawBase {_ _} _.
+Arguments RawLam {_ _} _ _.
+Arguments RawApp {_ _} _ _.
+
+(** ** Conversion of well-typed terms to named terms *)
+
+(**
+To do so, we need to assign to every variable a name.
+For that reason, we assign to every index in the context a name.
+ *)
+Inductive conNames {B : Type} (V : Type) : con B -> Type :=
+| EmptyNames : conNames V ∙
+| ExtendName : forall {A : ty B} {C : con B},
+    V -> conNames V C -> conNames V (A ,, C).
+
+Arguments EmptyNames {_ _}.
+Arguments ExtendName {_ _ _ _} _ _.
+
+Definition getName
+           {B V : Type}
+           {C : con B}
+           {A : ty B}
+           (names : conNames V C)
+           (v : var C A)
+  : V.
+Proof.
+  induction v.
+  - inversion names.
+    assumption.
+  - inversion names.
+    apply IHv.
+    assumption.
+Defined.
+
+(** We also need the length of contexts*)
+Fixpoint length {B : Type} (C : con B) : nat
+  := match C with
+     | ∙ => 0
+     | _ ,, C => S(length C)
+     end.
+
+(**
+To work with fresh variables, we assume that we can map natural numbers to variables.
+To each context, we can assign names by picking fresh variables.
+ *)
+Definition nameCon
+         {B : Type}
+         {V : Type}
+         (fresh : nat -> V)
+         (C : con B)
+         {n : nat}
+         (p : length C = n)
+  : conNames V C.
+Proof.
+  revert n p.
+  induction C ; intros n p.
+  - exact EmptyNames.
+  - simpl in p.
+    destruct n.
+    + discriminate.
+    + simple refine (ExtendName (fresh n) (IHC n _)).
+      inversion p.
+      reflexivity.
+Defined.
+
+(** ** Converting terms to well-typed terms *)
+Fixpoint tmToRawTm_help
+         {B F V : Type}
+         {ar : F -> ty B}
+         {C : con B}
+         {A : ty B}
+         (fresh : nat -> V)
+         (names : conNames V C)
+         {n : nat}
+         (p : n = length C)
+         (t : tm ar C A)
+  : rawTm V F
+  := match t with
+     | TmVar v => RawVar (getName names v)
+     | BaseTm f => RawBase f
+     | Lam f =>
+       let v := fresh n in
+       RawLam v (tmToRawTm_help fresh (ExtendName v names) (f_equal S p) f)
+     | App f t => RawApp (tmToRawTm_help fresh names p f) (tmToRawTm_help fresh names p t) 
+     end.
+
+Definition tmToRawTm
+           {B F V : Type}
+           {ar : F -> ty B}
+           {C : con B}
+           {A : ty B}
+           (fresh : nat -> V)
+           (t : tm ar C A)
+  : rawTm V F
+  := tmToRawTm_help fresh (nameCon fresh _ eq_refl) eq_refl t.
+
+(** * Printing afs *)
+
+(** To print an afs, we need the following data *)
+Record afs_show (S : Type) (B : Type) (V : Type) (F : Type) : Type :=
+  make_afs_show
+    {
+      (** Basic stuff *)
+      startTypes : S ;
+      startTerms : S ;
+      startRewrites : S ;
+      append : S -> S -> S ;
+      leftParen : S ;
+      rightParen : S ;
+      separate : S ;
+      empty : S ;
+      colon : S ;
+      fresh : nat -> V ;
+
+      (** Printing types *)
+      showBase : B -> S ;
+      arrow : S ;
+
+      (** Printing terms *)
+      showBaseFun : F -> S ;
+      showVars : V -> S ;
+      showLam : S ;
+      showLamSep : S ;
+      appSep : S ;
+
+      (** Rewrite rule *)
+      rewriteSym : S
+    }.
+
+Arguments startTypes {_ _ _ _} _.
+Arguments startTerms {_ _ _ _} _.
+Arguments startRewrites {_ _ _ _} _.
+
+Arguments append {_ _ _ _} _ _ _.
+Arguments leftParen {_ _ _ _} _.
+Arguments rightParen {_ _ _ _} _.
+Arguments empty {_ _ _ _} _.
+Arguments separate {_ _ _ _} _.
+Arguments colon {_ _ _ _} _.
+Arguments fresh {_ _ _ _} _ _.
+
+Arguments showBase {_ _ _ _} _ _.
+Arguments arrow {_ _ _ _} _.
+
+Arguments showBaseFun {_ _ _ _} _ _.
+Arguments showVars {_ _ _ _} _ _.
+Arguments showLam {_ _ _ _} _.
+Arguments showLamSep {_ _ _ _} _.
+Arguments appSep {_ _ _ _} _.
+
+Arguments rewriteSym {_ _ _ _} _.
+
+(** Showing list *)
+Fixpoint showList
+         {S B V F : Type}
+         (p : afs_show S B V F)
+         (l : list S)
+  : S
+  := match l with
+     | nil => empty p
+     | cons x xs => append p x (append p (separate p) (showList p xs))
+     end.
+
+(** Showing parentheses *)
+Definition showParen
+           {S B V F : Type}
+           (p : afs_show S B V F)
+           (s : S)
+  : S
+  := append p (append p (leftParen p) s) (rightParen p).
+
+(** Show function types *)
+Definition showFunctionType
+           {S B V F : Type}
+           (p : afs_show S B V F)
+           (s1 s2 : S)
+  : S
+  := append p s1 (append p (arrow p) s2).
+
+(** Showing types *)
+Fixpoint showType
+         {S B V F : Type}
+         (p : afs_show S B V F)
+         (A : ty B)
+  : S
+  := match A with
+     | Base b => showBase p b
+     | A1 ⟶ A2 => showFunctionType p (showOther p A1) (showType p A2)
+     end
+with showOther
+     {S B V F : Type}
+     (p : afs_show S B V F)
+     (A : ty B)
+  : S
+  := match A with
+     | Base b => showBase p b
+     | A1 ⟶ A2 => showParen p (showFunctionType p (showOther p A1) (showType p A2))
+     end.
+
+(** Showing terms *)
+Definition showApplication
+           {S B V F : Type}
+           (p : afs_show S B V F)
+           (s1 s2 : S)
+  : S
+  := append p s1 (append p (appSep p) s2).
+
+Definition showLambdaTm
+           {S B V F : Type}
+           (p : afs_show S B V F)
+           (v : V)
+           (s : S)
+  : S
+  := append
+       p
+       (showLam p)
+       (append
+          p
+          (showVars p v)
+          (append
+             p
+             (showLamSep p)
+             s)).
+
+Fixpoint showRawTm
+         {S B V F : Type}
+         (p : afs_show S B V F)
+         (t : rawTm V F)
+  : S
+  := match t with
+     | RawVar v => showVars p v
+     | RawBase f => showBaseFun p f
+     | RawApp t1 t2 => showApplication
+                         p
+                         (showRawTmApp p t1)
+                         (showRawTmVar p t2)
+     | RawLam v t => showLambdaTm p v (showRawTm p t)
+     end
+with showRawTmApp
+     {S B V F : Type}
+     (p : afs_show S B V F)
+     (t : rawTm V F)
+  : S
+  := match t with
+     | RawVar v => showVars p v
+     | RawBase f => showBaseFun p f
+     | RawApp t1 t2 => showApplication
+                         p
+                         (showRawTmApp p t1)
+                         (showRawTmVar p t2)
+     | RawLam v t => showParen p (showLambdaTm p v (showRawTm p t))
+     end
+with showRawTmVar
+     {S B V F : Type}
+     (p : afs_show S B V F)
+     (t : rawTm V F)
+  : S
+  := match t with
+     | RawVar v => showVars p v
+     | RawBase f => showBaseFun p f
+     | RawApp t1 t2 => showParen
+                         p
+                         (showApplication
+                            p
+                            (showRawTmApp p t1)
+                            (showRawTmVar p t2))
+     | RawLam v t => showParen p (showLambdaTm p v (showRawTm p t))
+     end.
+
+Definition showTm
+           {S B V F : Type}
+           (p : afs_show S B V F)
+           {ar : F -> ty B}
+           {C : con B}
+           {A : ty B}
+           (fresh : nat -> V)
+           (t : tm ar C A)
+  : S
+  := showRawTm p (tmToRawTm fresh t).
+  
+(** Showing an afs *)
+Definition show_afs_types
+           {S B V F : Type}
+           (p : afs_show S B V F)
+           (X : fin_afs B F)
+  : S
+  := append
+       p
+       (startTypes p)
+       (append
+          p
+          (separate p)
+          (showList p (map (showBase p) (@els _ (baseTyFin X))))).
+
+Definition show_function_symbol
+           {S B V F : Type}
+           (p : afs_show S B V F)
+           (X : fin_afs B F)
+           (f : F)
+  : S
+  := append
+       p
+       (showBaseFun p f)
+       (append
+          p
+          (colon p)
+          (showType p (arity X f))).
+
+Definition show_afs_functions
+           {S B V F : Type}
+           (p : afs_show S B V F)
+           (X : fin_afs B F)
+  : S
+  := append
+       p
+       (startTerms p)
+       (append
+          p
+          (separate p)
+          (showList
+             p
+             (map (show_function_symbol p X)
+                  (@els _ (baseTmFin X))))).
+
+Definition show_rewrite
+           {S B V F : Type}
+           (p : afs_show S B V F)
+           (X : fin_afs B F)
+           (r : rewriteRule (arity X))
+  : S
+  := append
+       p
+       (showTm p (fresh p) (lhs_of r))
+       (append
+          p
+          (rewriteSym p)
+          (showTm p (fresh p) (rhs_of r))).
+
+Definition show_afs_rewrites
+           {S B V F : Type}
+           (p : afs_show S B V F)
+           (X : fin_afs B F)
+  : S
+  := append
+       p
+       (startRewrites p)
+       (append
+          p
+          (separate p)
+          (showList p (map (show_rewrite p X) (list_of_rewriteRules X)))).
+
+Definition show_afs
+           {S B V F : Type}
+           (p : afs_show S B V F)
+           (X : fin_afs B F)
+  : S
+  := append
+       p
+       (show_afs_types p X)
+       (append
+          p
+          (append p (separate p) (show_afs_functions p X))
+          (append p (separate p) (show_afs_rewrites p X))).
+
+Fixpoint show_nat
+         (n : nat)
+  : string
+  := match n with
+     | 0 => ""
+     | S n => String.append "|" (show_nat n)
+     end.
+
+Definition string_printer : afs_show string string string string.
+Proof.
+  simple refine (make_afs_show _ _ _ _ _ _ _ _ _ _ _ _ _ _ _ _ _ _ _ _ _ _).
+  - exact "Types".
+  - exact "Terms".
+  - exact "Rewrite rules".
+  - exact String.append.
+  - exact "(".
+  - exact ")".
+  - exact "\n".
+  - exact "".
+  - exact ":".
+  - exact show_nat.
+  - exact (fun s => s).
+  - exact " -> ".
+  - exact (fun s => s).
+  - exact (fun s => s).
+  - exact "̈\\".
+  - exact ".".
+  - exact " ".
+  - exact "~>".
+Defined.
