Code/Syntax/StrongNormalization/BetaNormalForm.v
@@ -5,6 +5,8 @@ Require Import Syntax.Signature.
 Require Import Syntax.Signature.RewriteLemmas.
 Require Import Coq.Program.Equality.
 
+Local Open Scope type.
+
 (** * The definition of beta normal forms (for single step relation) *)
 Definition beta_nf
            {B : Type}
@@ -16,7 +18,6 @@ Definition beta_nf
   : Prop
   := nf (fun (t1 t2 : tm ar C A) => t1 ~>β t2) t.
 
-
 (** Relation between the two notions *)
 Proposition beta_nf_step
             {B : Type}
@@ -26,7 +27,7 @@ Proposition beta_nf_step
             {A : ty B}
             {t : tm ar C A}
             (Ht : beta_nf t)
-  : nf (fun (t1 t2 : tm ar C A) => t1 ~>β* t2) t.
+  : nf (fun (t1 t2 : tm ar C A) => t1 ~>β+ t2) t.
 Proof.
   intros t' r.
   induction r.
@@ -103,6 +104,25 @@ Proof.
   inversion b.
 Qed.
 
+Proposition beta_red_lam
+            {B : Type}
+            {F : Type}
+            {ar : F -> ty B}
+            {C : con B}
+            {A1 A2 : ty B}
+            {f : tm ar (A1 ,, C) A2}
+            {g : tm ar C (A1 ⟶ A2)}
+            (r : λ f ~>β g)
+  : { g' : tm ar (A1 ,, C) A2 & (f ~>β g') * (g = λ g') }.
+Proof.
+  dependent destruction r.
+  - exists f2.
+    split.
+    + exact r.
+    + reflexivity.
+  - inversion b.
+Qed.
+
 Proposition lam_beta_nf
             {B : Type}
             {F : Type}
@@ -133,6 +153,38 @@ Proof.
   refine (Hf (λ t') _).
   apply CLam.
   exact r.
+Qed.
+
+Proposition beta_red_app
+            {B : Type}
+            {F : Type}
+            {ar : F -> ty B}
+            {C : con B}
+            {A1 A2 : ty B}
+            {f : tm ar C (A1 ⟶ A2)}
+            {t : tm ar C A1}
+            {s : tm ar C A2}
+            (r : f · t ~>β s)
+  : { f' : tm ar C (A1 ⟶ A2) & (f ~>β f') * (s = f' · t) }
+    + { t' : tm ar C A1 & (t ~>β t') * (s = f · t') }
+    + { s' : tm ar C A2 & baseBetaStep _ _ (f · t) s' * (s = s') }.
+Proof.
+  dependent destruction r.
+  - do 2 left.
+    exists f2.
+    split.
+    + exact r.
+    + reflexivity.
+  - left ; right.
+    exists x2.
+    split.
+    + exact r.
+    + reflexivity.
+  - right.
+    exists t2.
+    split.
+    + exact b.
+    + reflexivity.
 Qed.
 
 Proposition app_beta_nf
@@ -411,7 +463,7 @@ Definition term_is_beta_SN
            {A : ty B}
            (t : tm ar C A)
   : Prop
-  := isWf (fun (t1 t2 : tm ar C _) => t1 ~>β* t2) t.
+  := isWf (fun (t1 t2 : tm ar C _) => t1 ~>β+ t2) t.
 
 Definition beta_nf_isSN
            {B : Type}
@@ -484,7 +536,7 @@ Proposition red_to_beta_SN
             {A : ty B}
             {t1 t2 : tm ar C A}
             (Ht : term_is_beta_SN t1)
-            (r : t1 ~>β* t2)
+            (r : t1 ~>β+ t2)
   : term_is_beta_SN t2.
 Proof.
   revert t2 r.
